example verifies using the prime versions of the type

examples/refinement/HighComp.fst
@@ -13,8 +13,12 @@ let comp a = state -> M (a * state)
 
 type hwp 'a = state -> ('a * state -> Type) -> Type
 
+// x:hwp a { monotonic x } 
+
 // [comp] type with wp
 type comp_wp 'a (wp : hwp 'a) = s0:state -> PURE ('a * state) (wp s0)
+
+type comp_wp' 'a (wp : hwp 'a) = s0:state -> PURE ('a * state) (wp s0)
 
 let comp_p (a:Type) (pre : state -> Type) (post : state -> a * state -> Type) : GTot Type  =
     s0:state -> Pure (a * state) (pre s0) (post s0)
@@ -27,6 +31,20 @@ unfold
 let bind_wp (wp1 : state -> ('a * state -> Type) -> Type)
             (wp2 : 'a -> state -> ('b * state -> Type) -> Type) : state -> ('b * state -> Type) -> Type =
             fun s0 post -> wp1 s0 (function (x, s1) -> wp2 x s1 post)
+
+unfold
+let trivial_pre = fun s0 -> True
+
+unfold
+let return_post (#a : Type) (x : a) = fun s0 r -> let (x1, s1) = r in x1 = x /\ s0 = s1
+
+unfold
+let bind_pre (#a : Type) (x : a) = fun s0 r -> let (x1, s1) = r in x1 = x /\ s0 = s1
+
+unfold
+let bind_post (#a : Type) (x : a) = fun s0 r -> let (x1, s1) = r in x1 = x /\ s0 = s1
+
+
 
 val hreturn : (a:Type) -> a -> comp a
 let hreturn (a:Type) (x : a) = fun s -> (x, s)
@@ -41,7 +59,7 @@ let hbind (a:Type) (b:Type) (m : comp a) (f : a -> comp b) =
 let hbind' (#a:Type) (#b:Type) (#wp1:hwp a) (#wp2:a -> hwp b) (m : comp_wp a wp1) (f : (x:a) -> comp_wp b (wp2 x)) :
   comp_wp b (bind_wp wp1 wp2) =
   fun s ->
-    admit (); // Probably due to a bug
+    admit (); 
     let (a, s1) = m s in
     f a s1
 
@@ -68,12 +86,6 @@ val hwrite' : i:nat -> v:mint -> comp_wp unit (write_wp i v)
 let hwrite' (i:nat) (v:mint) : comp_wp unit (write_wp i v) =
     fun s -> if i = 0 then ((), (v, snd s))
           else ((), (fst s, v))
-
-val dread : unit -> comp state
-let dread (_ : unit) : comp state = fun s -> (s, s)
-
-val dwrite : v:state -> comp unit
-let dwrite (v : state) : comp unit = fun s -> ((), v)
 
 // NOTE : ommiting type annotations from hread and hwrite defs
 // makes the effect definition fail
