examples/refinement/sum_and_swap.fst
@@ -15,12 +15,24 @@ let swap_and_sum () =
   hbind mint int (hread 1) (fun x1 -> 
   hbind unit int (hwrite 0 x1) (fun () -> 
   hbind unit int (hwrite 1 x0) (fun () ->
-  hbind mint int (hread 0) (fun x0' -> 
-  hreturn int (U32.v x0 + U32.v x1))))))
+  hreturn int (U32.v x0 + U32.v x1)))))
  
 
+// WP for sum and swap
 unfold
 let sum_wp : hwp int  = fun s0 post -> let (r1, r2) = s0 in post (U32.v r1 + U32.v r2, (r2, r1))
+
+// Pre and Post 
+unfold 
+let sum_pre = fun s0 -> True
+
+unfold 
+let sum_post = fun s0 res -> let (x, s1) = res in
+                          let (r1, r2) = s0 in 
+                          let (r1', r2') = s1 in 
+                          x = U32.v r1 + U32.v r2 /\
+                          r1 = r2' /\ r2 = r1'
+
 
 val hswap_and_sum : unit -> HIGH int sum_wp 
 let hswap_and_sum () = 
@@ -30,22 +42,23 @@ let hswap_and_sum () =
   let _  = HIGH?.put 1 x0 in
   U32.v x0 + U32.v x1
 
-// val swap_and_sum' : unit -> comp_wp int sum_wp 
-// let swap_and_sum' () =  
-//   hbind' (hread' 0) (fun x0 -> 
-//   hbind' (hread' 1) (fun x1 -> 
-//   hbind' (hwrite' 0 x1) (fun () -> 
-//   hbind' (hwrite' 1 x0) (fun () ->
-//   hbind' (hread' 0) (fun x0' -> 
-//   hreturn' (U32.v x0 + U32.v x1))))))
+val swap_and_sum' : unit -> comp_wp' int sum_wp 
+let swap_and_sum' () =  
+  hbind' (hread' 0) (fun x0 -> 
+  hbind' (hread' 1) (fun x1 -> 
+  hbind' (hwrite' 0 x1) (fun () ->
+  hbind' (hwrite' 1 x0) (fun () ->
+  hreturn' (U32.v x0 + U32.v x1)))))
 
 
-val lswap_and_sum : unit -> lcomp_wp int sum_wp (reif sum_wp hswap_and_sum)
+val lswap_and_sum : unit -> lcomp_wp' int sum_wp (reif sum_wp hswap_and_sum)
 let lswap_and_sum () =  
   lbind (lread 0) (fun x0 -> 
   lbind (lread 1) (fun x1 -> 
   lbind (lwrite 0 x1) (fun () -> 
   lbind (lwrite 1 x0) (fun () ->
-  lbind (lread 0) (fun x0' -> 
-  lreturn (U32.v x0 + U32.v x1))))))
+  lreturn (U32.v x0 + U32.v x1)))))
   
+// lemmas to comute reif and bind 
+// interm proof obligations remain provable in low comp
+// extend beyond seq composition with if and rec
